Sketch top-level proof of state_unthunk

compiler/backend/proofs/state_unthunkProofScript.sml
@@ -8,6 +8,7 @@ open stringTheory optionTheory sumTheory pairTheory listTheory alistTheory
      finite_mapTheory pred_setTheory rich_listTheory arithmeticTheory
 open pure_exp_lemmasTheory pure_miscTheory pure_configTheory
      stateLangTheory;
+local open pure_semanticsTheory in end
 
 val _ = new_theory "state_unthunkProof";
 
@@ -97,60 +98,236 @@ Inductive compile_rel:
 
 End
 
+Definition find_loc_def:
+  find_loc n [] = NONE ∧
+  find_loc n (x::xs) =
+    case x of
+    | NONE => if n = 0:num then SOME (0:num) else
+                OPTION_MAP (λn. n + 1:num) (find_loc (n-1) xs)
+    | SOME _ => OPTION_MAP (λn. n + 1:num) (find_loc n xs)
+End
+
 Inductive v_rel:
 
 [~Loc:]
-  (∀p st n1 n2.
-     FLOOKUP p n1 = SOME n2 ⇒
-     v_rel p st (Atom (Loc n1)) (Atom (Loc n2))) ∧
+  (∀p n1 n2.
+     find_loc n1 p = SOME n2 ⇒
+     v_rel p (Atom (Loc n1)) (Atom (Loc n2))) ∧
 
 [~Atom:]
-  (∀p st a.
+  (∀p a.
      (∀l. a ≠ Loc l) ⇒
-     v_rel p st (Atom a) (Atom a)) ∧
+     v_rel p (Atom a) (Atom a)) ∧
 
 [~Constructor:]
-  (∀p st tvs svs.
-     LIST_REL (v_rel p st) tvs svs ⇒
-     v_rel p st (Constructor s tvs) (Constructor s svs)) ∧
+  (∀p tvs svs.
+     LIST_REL (v_rel p) tvs svs ⇒
+     v_rel p (Constructor s tvs) (Constructor s svs)) ∧
 
 [~Closure:]
-  (∀p st tenv senv te se x.
-     env_rel p st tenv senv ∧
+  (∀p tenv senv te se x.
+     env_rel p tenv senv ∧
      compile_rel te se ⇒
-     v_rel p st (Closure x tenv te) (Closure x senv se)) ∧
+     v_rel p (Closure x tenv te) (Closure x senv se)) ∧
 
 [~Recclosure:]
-  (∀p st tenv senv tfns sfns n.
-     env_rel p st tenv senv ∧
+  (∀p tenv senv tfns sfns n.
+     env_rel p tenv senv ∧
      LIST_REL ((=) ### compile_rel) tfns sfns ⇒
-     v_rel p st (Recclosure tfns tenv n) (Recclosure sfns senv n)) ∧
+     v_rel p (Recclosure tfns tenv n) (Recclosure sfns senv n)) ∧
 
-[~Thunk_True:]
-  (∀p st tv sv n.
-     v_rel p st tv sv ∧
-     ~(n IN FRANGE p) ∧
-     oEL n st = SOME [True_v; sv] ⇒
-     v_rel p st (Thunk $ INL tv) (Atom (Loc n))) ∧
-
-[~Thunk_False:]
-  (∀tenv senv te se.
-     env_rel p st tenv senv ∧
-     compile_rel te se ∧
-     ~(n IN FRANGE p) ∧
-     oEL n st = SOME [False_v; Closure NONE senv se] ⇒
-     v_rel p st (Thunk $ INR (tenv, te)) (Atom (Loc n))) ∧
+[~Thunk:]
+  (∀p n r.
+     oEL n p = SOME (SOME r) ⇒
+     v_rel p (Thunk r) (Atom (Loc n))) ∧
 
 [env_rel:]
-  (∀p st tenv senv.
+  (∀p tenv senv.
      (∀n tv.
        ALOOKUP tenv n = SOME tv ⇒
-       ∃sv. ALOOKUP senv n = SOME sv ∧ v_rel p st tv sv) ⇒
-     env_rel p st tenv senv)
+       ∃sv. ALOOKUP senv n = SOME sv ∧ v_rel p tv sv) ⇒
+     env_rel p tenv senv)
 
 End
 
-Theorem env_rel_def = “env_rel p st tenv senv”
+Theorem env_rel_def = “env_rel p tenv senv”
   |> SIMP_CONV (srw_ss()) [Once v_rel_cases];
+
+Inductive step_res_rel:
+  (v_rel p v1 v2 ⇒
+   step_res_rel p (Val v1) (Val v2)) ∧
+  (v_rel p v1 v2 ⇒
+   step_res_rel p (Exn v1) (Exn v2)) ∧
+  (compile_rel e1 e2 ∧ env_rel p env1 env2 ⇒
+   step_res_rel p (Exp env1 e1) (Exp env2 e2)) ∧
+  (step_res_rel p (Action a b) (Action a b))
+End
+
+Inductive cont_rel:
+  ∀xs. xs = [] ⇒ cont_rel p xs []
+End
+
+Definition state_rel_def:
+  state_rel (p:(v + env # exp) option list) (ts:state option) (ss:state option) = T
+End
+
+Inductive snext_res_rel:
+  (state_rel p (SOME ts) (SOME ss) ∧ cont_rel p tk sk ⇒
+   snext_res_rel p (Act x tk (SOME ts)) (Act x sk (SOME ss))) ∧
+  (snext_res_rel p Ret Ret) ∧
+  (snext_res_rel p Div Div) ∧
+  (snext_res_rel p Err Err)
+End
+
+Theorem step_n_is_halt_SOME:
+  step_n n (tr,SOME ts,tk) = (tr1,ts1,tk1) ∧ is_halt (tr1,ts1,tk1) ∧ tr1 ≠ Error ⇒
+  ∃ts2. ts1 = SOME ts2
+Proof
+  cheat
+QED
+
+Theorem step_forward:
+  ∀n p tr ts tk tr1 ts1 tk1 ss sr sk.
+    step_n n (tr,ts,tk) = (tr1,ts1,tk1) ∧ is_halt (tr1,ts1,tk1) ∧
+    cont_rel p tk sk ∧
+    state_rel p ts (SOME ss) ∧
+    step_res_rel p tr sr ∧ tr1 ≠ Error ⇒
+    ∃m q sr1 ss1 sk1.
+      step_n m (sr,SOME ss,sk) = (sr1,SOME ss1,sk1) ∧
+      is_halt (sr1,SOME ss1,sk1) ∧
+      cont_rel q tk1 sk1 ∧
+      state_rel q ts1 (SOME ss1) ∧
+      step_res_rel q tr1 sr1
+Proof
+  cheat
+QED
+
+Theorem step_backward:
+  ∀m p sr ss sk sr1 ss1 sk1 tr ts tk.
+    step_n m (sr,SOME ss,sk) = (sr1,ss1,sk1) ∧
+    is_halt (sr1,ss1,sk1) ∧
+    cont_rel p tk sk ∧
+    state_rel p ts (SOME ss) ∧
+    step_res_rel p tr sr ⇒
+    ∃n q tr1 ts1 tk1.
+      step_n n (tr,ts,tk) = (tr1,ts1,tk1) ∧
+      is_halt (tr1,ts1,tk1)
+Proof
+  cheat
+QED
+
+(* step_until_halt *)
+
+Theorem step_until_halt_thm:
+  step_res_rel p tr sr ∧
+  state_rel p (SOME ts) (SOME ss) ∧
+  cont_rel p tk sk ∧
+  step_until_halt (tr,SOME ts,tk) ≠ Err ⇒
+  ∃q. snext_res_rel q (step_until_halt (tr,SOME ts,tk))
+                      (step_until_halt (sr,SOME ss,sk))
+Proof
+  fs [step_until_halt_def]
+  \\ DEEP_INTRO_TAC some_intro \\ fs [] \\ rw []
+  >-
+   (‘∃a. step_n x (tr,SOME ts,tk) = a’ by fs []
+    \\ PairCases_on ‘a’ \\ gvs []
+    \\ ‘a0 ≠ Error’ by (strip_tac \\ gvs [])
+    \\ drule_all step_forward \\ rw []
+    \\ reverse (DEEP_INTRO_TAC some_intro \\ fs [] \\ rw [])
+    >- metis_tac []
+    \\ ‘step_n x' (sr,SOME ss,sk) = step_n m (sr,SOME ss,sk)’
+      by metis_tac [is_halt_imp_eq]
+    \\ gvs []
+    \\ qpat_x_assum ‘step_res_rel _ _ _’ mp_tac
+    \\ simp [Once step_res_rel_cases] \\ strip_tac \\ gvs []
+    \\ simp [Once snext_res_rel_cases] \\ gvs []
+    \\ rpt (first_assum $ irule_at Any)
+    \\ qpat_x_assum ‘step_n x _ = _’ assume_tac
+    \\ drule step_n_is_halt_SOME \\ gvs []
+    \\ strip_tac \\ gvs [])
+  \\ reverse (DEEP_INTRO_TAC some_intro \\ fs [] \\ rw [])
+  >- simp [Once snext_res_rel_cases]
+  \\ ‘∃a. step_n x (sr,SOME ss,sk) = a’ by fs []
+  \\ PairCases_on ‘a’ \\ gvs []
+  \\ drule_all step_backward
+  \\ metis_tac []
+QED
+
+(* unfold *)
+
+Theorem semantics_thm:
+  compile_rel e1 e2 ∧
+  state_rel p (SOME ts) (SOME ss) ∧
+  env_rel p tenv senv ∧
+  cont_rel p tk sk ⇒
+  semantics e1 tenv (SOME ts) tk --->
+  semantics e2 senv (SOME ss) sk
+Proof
+  qsuff_tac ‘
+    ∀t1 t2.
+      (∃p e1 e2 ts ss tenv senv tk sk.
+        compile_rel e1 e2 ∧
+        state_rel p (SOME ts) (SOME ss) ∧
+        env_rel p tenv senv ∧
+        cont_rel p tk sk ∧
+        t1 = semantics e1 tenv (SOME ts) tk ∧
+        t2 = semantics e2 senv (SOME ss) sk) ⇒
+      t1 ---> t2’
+  >- (rw [PULL_EXISTS]
+      \\ last_x_assum drule
+      \\ rpt (disch_then drule) \\ fs [])
+  \\ ho_match_mp_tac pure_semanticsTheory.compiles_to_coind
+  \\ rpt gen_tac \\ strip_tac
+  \\ ntac 2 (pop_assum $ mp_tac o GSYM)
+  \\ simp [stateLangTheory.semantics_def]
+  \\ simp [Once sinterp_def] \\ strip_tac
+  \\ simp [Once sinterp_def] \\ strip_tac
+  \\ ntac 2 $ pop_assum mp_tac
+  \\ once_rewrite_tac [io_treeTheory.io_unfold_err]
+  \\ fs []
+  \\ simp [GSYM sinterp_def]
+  \\ Cases_on ‘step_until_halt (Exp tenv e1,SOME ts,tk) = Err’ >- fs []
+  \\ drule_at (Pos last) step_until_halt_thm
+  \\ rpt (disch_then $ drule_at $ Pos last)
+  \\ disch_then $ qspec_then ‘Exp senv e2’ mp_tac
+  \\ impl_tac
+  >- simp [Once step_res_rel_cases]
+  \\ rename [‘snext_res_rel _ xx yy’]
+  \\ simp [snext_res_rel_cases]
+  \\ strip_tac \\ fs []
+  \\ rw [] \\ gvs []
+  \\ Cases \\ fs []
+  \\ IF_CASES_TAC \\ fs []
+  \\ fs [] \\ fs [value_def] \\ rw []
+  \\ simp [sinterp_def]
+  \\ ‘compile_rel (Lit (Str y)) (Lit (Str y))’ by simp [Once compile_rel_cases]
+  \\ pop_assum $ irule_at Any
+  \\ qpat_x_assum ‘cont_rel _ _ _’ $ irule_at Any
+  \\ ‘env_rel q [] []’ by fs [env_rel_def]
+  \\ pop_assum $ irule_at Any
+  \\ qpat_x_assum ‘state_rel q _ _’ $ irule_at Any
+  \\ simp [value_def]
+  \\ once_rewrite_tac [io_treeTheory.io_unfold_err]
+  \\ rpt conj_tac
+  \\ rpt AP_THM_TAC
+  \\ fs []
+  \\ AP_TERM_TAC
+  \\ rpt AP_THM_TAC
+  \\ AP_TERM_TAC
+  \\ once_rewrite_tac [EQ_SYM_EQ]
+  \\ irule step_unitl_halt_unwind
+  \\ fs [step_def,application_def,get_atoms_def,value_def]
+QED
+
+Theorem compile_rel_itree_of:
+  compile_rel e1 e2 ⇒
+  itree_of e1 ---> itree_of e2
+Proof
+  fs [stateLangTheory.itree_of_def] \\ rw []
+  \\ irule semantics_thm
+  \\ simp [Once cont_rel_cases]
+  \\ fs [env_rel_def]
+  \\ qexists_tac ‘[]’ \\ fs [state_rel_def]
+QED
 
 val _ = export_theory ();
